Reproved system calls in the setting of key injections
proof is very quick and dirt, still needs cleanup

needed to prove lemmas about refinement relations being preserved by
key injection extension

needed to rephrase the mkkey_fresh hypothesis and mkkey step rule, the
new list of keys is just the cons of the old list and the new key

using ssreflect eqType for abstract keys :)

sealing/abstract.v
@@ -1,6 +1,7 @@
 Require Import List. Import ListNotations.
 Require Import Coq.Bool.Bool.
 Require Import Coq.Classes.SetoidDec.
+Require Import ssreflect eqtype.
 Require Import lib.utils.
 
 Import DoNotation.
@@ -22,15 +23,13 @@ Context (t : machine_types)
         {ssa : @sealing_syscall_addrs t}.
 
 Class sealing_key := {
-  key       : Type;
+  key       : eqType;
 
   (* This function is total, so sym_key has to be infinite *)
-  mkkey_f : list key -> (list key) * key;
+  mkkey_f : list key -> key;
  
   (* This ensures freshness without fixing a generation strategy *)
-  mkkey_fresh : forall ks ks' k,
-                  mkkey_f ks = (ks', k) ->
-                  ~In k ks /\ In k ks' /\ incl ks ks'
+  mkkey_fresh : forall ks, ~In (mkkey_f ks) ks
 }.
 
 Context {sk : sealing_key}.
@@ -69,84 +68,83 @@ Definition decode (mem : memory) (pc : word t) :=
   end.
 
 Inductive step (st st' : state) : Prop :=
-| step_nop : forall mem reg pc es
-    (ST   : st = State mem reg pc es)
+| step_nop : forall mem reg pc ks
+    (ST   : st = State mem reg pc ks)
     (INST : decode mem pc =? Nop _)
-    (NEXT : st' = State mem reg (pc.+1) es),   step st st'
-| step_const : forall mem reg reg' pc n r es
-    (ST   : st = State mem reg pc es)
+    (NEXT : st' = State mem reg (pc.+1) ks),   step st st'
+| step_const : forall mem reg reg' pc n r ks
+    (ST   : st = State mem reg pc ks)
     (INST : decode mem pc =? Const _ n r)
     (UPD  : upd reg r (VData (imm_to_word n)) =? reg')
-    (NEXT : st' = State mem reg' (pc.+1) es),   step st st'
-| step_mov : forall mem reg reg' pc r1 v1 r2 es
-    (ST   : st = State mem reg pc es)
+    (NEXT : st' = State mem reg' (pc.+1) ks),   step st st'
+| step_mov : forall mem reg reg' pc r1 v1 r2 ks
+    (ST   : st = State mem reg pc ks)
     (INST : decode mem pc =? Mov _ r1 r2)
     (R1W  : get reg r1 =? v1)
     (UPD  : upd reg r2 v1 =? reg')
-    (NEXT : st' = State mem reg' (pc.+1) es),   step st st'
-| step_binop : forall mem reg reg' pc op r1 r2 r3 w1 w2 es
-    (ST   : st = State mem reg pc es)
+    (NEXT : st' = State mem reg' (pc.+1) ks),   step st st'
+| step_binop : forall mem reg reg' pc op r1 r2 r3 w1 w2 ks
+    (ST   : st = State mem reg pc ks)
     (INST : decode mem pc =? Binop _ op r1 r2 r3)
     (R1W  : get reg r1 =? VData w1)
     (R2W  : get reg r2 =? VData w2)
     (UPD  : upd reg r3 (VData (binop_denote op w1 w2)) =? reg')
-    (NEXT : st' = State mem reg' (pc.+1) es),   step st st'
-| step_load : forall mem reg reg' pc r1 r2 w1 v2 es
-    (ST   : st = State mem reg pc es)
+    (NEXT : st' = State mem reg' (pc.+1) ks),   step st st'
+| step_load : forall mem reg reg' pc r1 r2 w1 v2 ks
+    (ST   : st = State mem reg pc ks)
     (INST : decode mem pc =? Load _ r1 r2)
     (R1W  : get reg r1 =? VData w1)
     (MEM1 : get mem w1 =? v2)
     (UPD  : upd reg r2 v2 =? reg')
-    (NEXT : st' = State mem reg' (pc.+1) es),   step st st'
-| step_store : forall mem mem' reg pc r1 r2 w1 v2 es
-    (ST   : st = State mem reg pc es)
+    (NEXT : st' = State mem reg' (pc.+1) ks),   step st st'
+| step_store : forall mem mem' reg pc r1 r2 w1 v2 ks
+    (ST   : st = State mem reg pc ks)
     (INST : decode mem pc =? Store _ r1 r2)
     (R1W  : get reg r1 =? VData w1)
     (R2W  : get reg r2 =? v2)
     (UPDM : upd mem w1 v2 =? mem')
-    (NEXT : st' = State mem' reg (pc.+1) es),   step st st'
-| step_jump : forall mem reg pc r w es
-    (ST   : st = State mem reg pc es)
+    (NEXT : st' = State mem' reg (pc.+1) ks),   step st st'
+| step_jump : forall mem reg pc r w ks
+    (ST   : st = State mem reg pc ks)
     (INST : decode mem pc =? Jump _ r)
     (RW   : get reg r =? VData w)
-    (NEXT : st' = State mem reg w es),   step st st'
-| step_bnz : forall mem reg pc r n w es
-    (ST   : st = State mem reg pc es)
+    (NEXT : st' = State mem reg w ks),   step st st'
+| step_bnz : forall mem reg pc r n w ks
+    (ST   : st = State mem reg pc ks)
     (INST : decode mem pc =? Bnz _ r n)
     (RW   : get reg r =? VData w),
     let pc' := add_word pc (if w ==b Z_to_word 0
                             then Z_to_word 1 else imm_to_word n) in forall
-    (NEXT : st' = State mem reg pc' es),   step st st'
-| step_jal : forall mem reg reg' pc r w es
-    (ST   : st = State mem reg pc es)
+    (NEXT : st' = State mem reg pc' ks),   step st st'
+| step_jal : forall mem reg reg' pc r w ks
+    (ST   : st = State mem reg pc ks)
     (INST : decode mem pc =? Jal _ r)
     (RW   : get reg r =? VData w)
     (NOSC : ~In w syscall_addrs)
     (UPD  : upd reg ra (VData (pc.+1)) =? reg')
-    (NEXT : st' = State mem reg' w es),   step st st'
-| step_mkkey : forall mem reg reg' pc r es es' nk
-    (ST   : st = State mem reg pc es)
+    (NEXT : st' = State mem reg' w ks),   step st st'
+| step_mkkey : forall mem reg reg' pc r ks
+    (ST   : st = State mem reg pc ks)
     (INST : decode mem pc =? Jal _ r)
     (RW   : get reg r =? VData mkkey_addr)
-    (GEN  : mkkey_f es = (es',nk))
-    (UPD  : upd reg syscall_ret (VKey nk) =? reg')
-    (NEXT : st' = State mem reg' pc es'),   step st st'
-| step_seal : forall mem reg reg' pc r es payload key
-    (ST   : st = State mem reg pc es)
+    (UPD  : upd reg syscall_ret (VKey (mkkey_f ks)) =? reg')
+    (NEXT : st' = State mem reg' pc ((mkkey_f ks) :: ks)),   step st st'
+| step_seal : forall mem reg reg' pc r ks payload key
+    (ST   : st = State mem reg pc ks)
     (INST : decode mem pc =? Jal _ r)
     (RW   : get reg r =? VData seal_addr)
     (R1   : get reg syscall_arg1 =? VData payload)
     (R2   : get reg syscall_arg2 =? VKey key)
     (UPD  : upd reg syscall_ret (VSealed payload key) =? reg')
-    (NEXT : st' = State mem reg' pc es),   step st st'
-| step_unseal : forall mem reg reg' pc r es payload key
-    (ST   : st = State mem reg pc es)
+    (NEXT : st' = State mem reg' pc ks),   step st st'
+| step_unseal : forall mem reg reg' pc r ks payload key
+    (ST   : st = State mem reg pc ks)
     (INST : decode mem pc =? Jal _ r)
     (RW   : get reg r =? VData unseal_addr)
     (R1   : get reg syscall_arg1 =? VSealed payload key)
     (R2   : get reg syscall_arg2 =? VKey key)
     (UPD  : upd reg syscall_ret (VData payload) =? reg')
-    (NEXT : st' = State mem reg' pc es),   step st st'.
+    (NEXT : st' = State mem reg' pc ks),   step st st'.
 
 End WithClasses.
 
